git-svn-id: https://svn-agbkb.informatik.uni-bremen.de/Hets-lib/trunk@1247 9acf5e20-c632-0410-b30d-e55f0e25a569

Isabelle/ISO/Nat_monadic.thy
@@ -1,13 +1,13 @@
 theory Nat_monadic
-imports "$HETS_LIB/Isabelle/MainHC"
-uses "$HETS_LIB/Isabelle/prelude"
+imports "$HETS_LIB/Isabelle/MainHC" "Primes" "Parity"
+uses "$HETS_LIB/Isabelle/prelude" 
 begin
 
 ML "Header.initialize
     [\"ga_selector_pre\", \"ga_injective_suc\", \"ga_disjoint_0_suc\",
      \"ga_selector_undef_pre_0\", \"X1_def_Nat\", \"X2_def_Nat\",
-     \"X4_def_Nat\", \"X5_def_Nat\", \"X6_def_Nat\", \"X7_def_Nat\",
-     \"X8_def_Nat\", \"X9_def_Nat\", \"decimal_def\",
+     \"X3_def_Nat\", \"X4_def_Nat\", \"X5_def_Nat\", \"X6_def_Nat\",
+     \"X7_def_Nat\", \"X8_def_Nat\", \"X9_def_Nat\", \"decimal_def\",
      \"ga_comm___XPlus__\", \"ga_assoc___XPlus__\",
      \"ga_right_unit___XPlus__\", \"ga_left_unit___XPlus__\",
      \"ga_left_comm___XPlus__\", \"ga_comm___Xx__\",
@@ -61,6 +61,18 @@ X_min :: "X_Nat => X_Nat => X_Nat" ("min''/'(_,/ _')" [3,3] 999)
 X_odd :: "X_Nat => bool" ("odd''/'(_')" [3] 999)
 X_pre :: "X_Nat => X_Nat partial" ("pre/'(_')" [3] 999)
 
+section "Extension of Naturals"
+(* we introduce some new symbols *)
+consts combine_nat :: "nat => nat => nat" ("(_/ @@@/ _)" [54,54] 52)
+consts part_div :: "nat => nat => nat partial" ("(_/ '/??/ _)" [54,54] 52)
+consts part_minus :: "nat => nat => nat partial" ("(_/ '-??/ _)" [54,54] 52)
+
+primrec pre_nat
+where
+  pre_nat_0: "pre_nat 0 = noneOp"
+  | pre_nat_suc: "pre_nat (Suc n) = makePartial n"
+
+
 axioms
 ga_selector_pre [rule_format] :
 "ALL XX1. pre(suc(XX1)) = makePartial XX1"
@@ -75,6 +87,8 @@ ga_selector_undef_pre_0 [rule_format] : "~ defOp (pre(0'))"
 X1_def_Nat [rule_format] : "1' = suc(0')"
 
 X2_def_Nat [rule_format] : "2' = suc(1')"
+
+X3_def_Nat [rule_format] : "3' = suc(2')"
 
 X4_def_Nat [rule_format] : "4' = suc(3')"
 
@@ -249,6 +263,16 @@ div_mod_Nat [rule_format] :
 power_Nat [rule_format] :
 "ALL m. ALL r. ALL s. m ^' (r +' s) = (m ^' r) *' (m ^' s)"
 
+decimal_def_nat [rule_format] : 
+"ALL m. ALL X_n. m @@@ X_n = (m * Suc(9)) + X_n"
+
+divide_Pos_nat [rule_format] :
+"ALL m. ALL X_n. ALL r. X_n > 0 --> m /?? X_n = makePartial r = (m = r * X_n)"
+
+part_div_def : "x /??y = (if (x mod y = 0) then makePartial(x div y) else noneOp)"
+part_minus_def : "x -?? y = (if (x>=y) then makePartial(x-y) else noneOp)"
+
+
 declare ga_selector_pre [simp]
 declare ga_selector_undef_pre_0 [simp]
 declare ga_comm___XPlus__ [simp]
@@ -292,5 +316,600 @@ declare subTotal_def2_Nat [simp]
 declare sub_dom_Nat [simp]
 declare divide_0_Nat [simp]
 declare min_0 [simp]
+
+lemma makePartialproj[simp]: "makeTotal(makePartial x)=x"
+apply (subst makeTotal_def)
+apply (subst makePartial_def)
+apply (auto)
+done
+
+primrec Nat2nat
+where 
+  Nat2nat_0: "Nat2nat  0' = 0 " 
+  | Nat2nat_suc: "Nat2nat  (X_suc x) = Suc (Nat2nat x)"
+
+
+primrec nat2Nat
+where
+  nat2Nat_0: "nat2Nat 0 = 0'"
+| nat2Nat_Suc: "nat2Nat (Suc x) = X_suc (nat2Nat x)"
+
+lemma iso1 [simp] : "! x . nat2Nat(Nat2nat x) = x"
+apply (auto)
+apply (induct_tac x)
+apply (auto)
+done
+
+lemma iso2 [simp] : "! x. Nat2nat(nat2Nat x) = x"
+apply (auto)
+apply (induct_tac x)
+apply (auto)
+done
+
+
+lemma nat2Nat_injectivity : "nat2Nat(x) = nat2Nat(y) ==> x = y"
+apply (drule_tac f="%x. Nat2nat(x)" in arg_cong)
+apply (simp)
+done
+
+lemma Nat2nat_injectivity : "Nat2nat(x) = Nat2nat(y) ==>  x = y"
+apply (drule_tac f="%x. nat2Nat(x)" in arg_cong)
+apply (simp)
+done
+
+lemma nat2Nat_injectivity_negated : "nat2Nat(x) ~= nat2Nat(y) ==> x ~= y"
+apply (auto)
+done
+
+lemma Nat2nat_injectivity_negated : "Nat2nat(x) ~= Nat2nat(y) ==>  x ~= y"
+apply (auto)
+done
+
+(* ask Lutz which version to use *)
+lemma inj_predefined : "inj Nat2nat"
+apply (simp add: inj_on_def)
+apply (auto)
+apply (drule_tac f="%x. nat2Nat(x)" in arg_cong)
+apply (simp)
+done
+
+section "Simple Definitions"
+
+(* the numbers need special treatment. we use the following strategy: 1' is manually proved
+   for subsequent numbers: apply definition for n' -> suc( [n-1]'), use theorem for [n-1]', ripple out via nat2Nat_Suc *)
+
+(* ============================== 1 ============================== *)
+
+(*by (auto simp add: X1_def_Nat)*)
+theorem nat2Nat_1_def_Nat[simp] : "nat2Nat(1) = 1'"
+apply (simp)
+apply (subst X1_def_Nat)
+apply (auto)
+done
+
+(* get backwards direction via the iso (already in the simplifier) and the other direction *)
+theorem Nat2nat_1_def_Nat[simp] : "Nat2nat(1')=1"
+apply (simp add: nat2Nat_1_def_Nat[THEN sym])
+done
+
+(* ============================== 2 ============================== *)
+
+theorem nat2Nat_2_def_Nat[simp] : "nat2Nat(2) =2'"
+apply (subst X2_def_Nat)
+apply (subst nat2Nat_1_def_Nat[THEN sym])
+apply (subst nat2Nat_Suc [rule_format, THEN sym])
+apply (subgoal_tac "Suc 1 = 2")
+apply (drule_tac f="%x. nat2Nat(x)" in arg_cong)
+apply (auto)
+done
+
+theorem two_2[simp]  : "Nat2nat(2') = 2"
+apply (subst nat2Nat_2_def_Nat[THEN sym])
+apply (simp only: iso2)
+done
+
+(* ============================== 3 ============================== *)
+
+theorem nat2Nat_3_def_Nat[simp] : "nat2Nat(3) = 3'"
+apply (subst X3_def_Nat)
+apply (subst nat2Nat_2_def_Nat[THEN sym])
+apply (subst nat2Nat_Suc [rule_format, THEN sym])
+apply (simp)
+done
+
+theorem nat2Nat_3_def_nat[simp] : "Nat2nat(3') = 3"
+apply (subst nat2Nat_3_def_Nat[THEN sym])
+apply (simp only: iso2)
+done
+
+(* ============================== 4 ============================== *)
+
+theorem nat2Nat_4_def_Nat[simp] : "nat2Nat(4) = 4'"
+apply (subst X4_def_Nat)
+apply (subst nat2Nat_3_def_Nat[THEN sym])
+apply (subst nat2Nat_Suc [rule_format, THEN sym])
+apply (simp)
+done
+
+theorem Nat2nat_4_def_Nat : "Nat2nat(4') = 4"
+apply (subst nat2Nat_4_def_Nat[THEN sym])
+apply (simp only: iso2)
+done
+
+(* ============================== 5 ============================== *)
+
+theorem nat2Nat_5_def_Nat[simp] : "nat2Nat(5) = 5'"
+apply (subst X5_def_Nat)
+apply (subst nat2Nat_4_def_Nat[THEN sym])
+apply (subst nat2Nat_Suc [rule_format, THEN sym])
+apply (simp)
+done
+
+theorem Nat2nat_5_def_Nat[simp] : "Nat2nat(5') = 5"
+apply (subst nat2Nat_5_def_Nat[THEN sym])
+apply (simp only: iso2)
+done
+
+(* ============================== 6 ============================== *)
+
+theorem nat2Nat_6_def_Nat[simp] : "nat2Nat(6) = 6'"
+apply (subst X6_def_Nat)
+apply (subst nat2Nat_5_def_Nat[THEN sym])
+apply (subst nat2Nat_Suc [rule_format, THEN sym])
+apply (simp)
+done
+
+theorem Nat2nat_6_def_Nat[simp] : "Nat2nat(6') = 6"
+apply (subst nat2Nat_6_def_Nat[THEN sym])
+apply (simp only: iso2)
+done
+
+(* ============================== 7 ============================== *)
+
+theorem nat2Nat_7_def_Nat[simp] : "nat2Nat(7)=7'"
+apply (subst X7_def_Nat)
+apply (subst nat2Nat_6_def_Nat[THEN sym])
+apply (subst nat2Nat_Suc [rule_format, THEN sym])
+apply (simp)
+done
+
+theorem Nat2nat_7_def_Nat[simp] : "Nat2nat(7') = 7"
+apply (subst nat2Nat_7_def_Nat[THEN sym])
+apply (simp only: iso2)
+done
+
+(* ============================== 8 ============================== *)
+
+theorem nat2Nat_8_def_Nat[simp] : "nat2Nat(8) = 8'"
+apply (subst X8_def_Nat)
+apply (subst nat2Nat_7_def_Nat[THEN sym])
+apply (subst nat2Nat_Suc [rule_format, THEN sym])
+apply (simp)
+done
+
+theorem Nat2nat_8_def_Nat[simp] : "Nat2nat(8') = 8 "
+apply (subst nat2Nat_8_def_Nat[THEN sym])
+apply (simp only: iso2)
+done
+
+(* ============================== 9 ============================== *)
+
+theorem nat2Nat_9_def_Nat[simp] : "nat2Nat(9) = 9'"
+apply (subst X9_def_Nat)
+apply (subst nat2Nat_8_def_Nat[THEN sym])
+apply (subst nat2Nat_Suc [rule_format, THEN sym])
+apply (simp)
+done
+
+theorem Nat2nat_9_def_Nat[simp] : "Nat2nat(9') = 9"
+apply (subst nat2Nat_9_def_Nat[THEN sym])
+apply (simp only: iso2)
+done
+
+
+section "Recursive Definitions"
+
+theorem nat2Nat_add [simp] : "nat2Nat (x + y) = (nat2Nat x) +' (nat2Nat y)"
+apply (induct_tac x)
+apply (auto simp only: nat2Nat_Suc nat2Nat_0 add_Suc add_0 add_suc_Nat add_0_Nat)
+done
+
+theorem Nat2nat_add[simp] : "Nat2nat (x +' y) = (Nat2nat x) + (Nat2nat y)"
+apply (rule nat2Nat_injectivity)
+apply (auto)
+done
+
+theorem nat2Nat_mul [simp] : "nat2Nat (x * y) = (nat2Nat x) *' (nat2Nat y)"
+apply (induct_tac x)
+apply (auto simp only: nat2Nat_Suc nat2Nat_0 nat2Nat_add mult_Suc mult_0 mult_suc_Nat mult_0_Nat)
+apply (auto)
+done
+
+theorem Nat2nat_mul [simp] : "Nat2nat (x *' y) = (Nat2nat x) * (Nat2nat y)"
+apply (rule nat2Nat_injectivity)
+apply (auto)
+done
+
+theorem nat2Nat_power [simp] : "nat2Nat(x ^ y) = nat2Nat(x) ^' nat2Nat(y)"
+apply (induct_tac y)
+apply (auto)
+apply (simp add: X1_def_Nat)
+done
+
+theorem Nat2nat_power [simp]: "Nat2nat(x ^' y) = Nat2nat(x) ^ Nat2nat(y)"
+apply (rule nat2Nat_injectivity)
+apply (auto)
+done
+
+theorem nat2Nat_fac [simp] : "nat2Nat(fact(x)) = nat2Nat(x)!'"
+apply (induct_tac x)
+apply (simp add: X1_def_Nat)
+apply (subst fact.simps)
+apply (simp only: nat2Nat_mul nat2Nat_Suc factorial_suc)
+done
+
+theorem Nat2nat_fac [simp] : "Nat2nat(x!') = fact(Nat2nat(x))"
+apply (rule nat2Nat_injectivity)
+apply auto
+done
+
+section "Predicates"
+
+
+subsection "ordering"
+
+lemma no_le_zero [simp] : "(x <=' 0') = (x = 0')"
+apply (case_tac x)
+by (auto)
+
+lemma no_nat2Nat_zero [simp] : "!!x. nat2Nat x = 0' ==> x = 0"
+apply (rule nat2Nat_injectivity)
+apply simp
+done
+
+theorem nat2Nat_lt_equal [simp] : "nat2Nat(x) <=' nat2Nat(y) <->x <= y "
+apply (rule diff_induct)
+apply (auto)
+done
+
+theorem Nat2nat_lt_equal [simp] : "(Nat2nat(x) <= Nat2nat(y)) <-> (x <=' y)"
+apply (subst nat2Nat_lt_equal[THEN sym])
+apply (simp only: iso1)
+done
+
+theorem nat2Nat_lt [simp] : "nat2Nat(x) <' nat2Nat(y) <-> x < y"
+apply (rule diff_induct)
+apply (auto)
+done
+
+theorem Nat2nat_lt [simp] : "Nat2nat(x) < Nat2nat(y) <-> x <' y"
+apply (subst nat2Nat_lt[THEN sym])
+apply (simp only: iso1)
+done
+
+theorem nat2Nat_gt [simp] : " nat2Nat(x) >' nat2Nat(y) <-> x > y"
+apply (rule diff_induct)
+apply (auto)
+done
+
+theorem Nat2nat_gt [simp] : "Nat2nat(x) > Nat2nat(y) <-> x >' y "
+apply (subst nat2Nat_gt[THEN sym])
+apply (simp)
+done
+
+theorem nat2Nat_gt_equal [simp] : "nat2Nat(x) >=' nat2Nat(y) <-> x >= y"
+apply (rule diff_induct)
+apply (auto)
+done
+
+theorem Nat2nat_gt_equal [simp] : "Nat2nat(x) >= Nat2nat(y) <-> x >=' y"
+apply (subst nat2Nat_gt_equal[THEN sym])
+apply(auto)
+done
+
+subsection "Even and Odd"
+
+lemma suc_even_nat: "even(x) ==> even(Suc(Suc(x)))"
+apply (auto)
+done
+
+theorem nat2Nat_even [simp] : "((even(Nat2nat(x)) <-> even'(x)) & (odd(Nat2nat(x)) <-> odd'(x)))"
+apply (induct x)
+apply (simp)
+apply (rule conjI)
+apply (simp)
+apply (simp)
+done
+
+theorem Nat2nat_even [simp] : "(even'(nat2Nat(x)) <-> (even(x)) & (odd'(nat2Nat(x)) <-> odd(x)))"
+apply (insert nat2Nat_even [of "nat2Nat(x)"])
+apply (auto)
+done
+
+theorem nat2Nat_dvd [simp] : "(nat2Nat(x) dvd' nat2Nat(y)) <-> (x dvd y)"
+apply (subst dvd_def_Nat)
+apply (subst dvd_def)
+apply (rule iffI)
+apply (simp)
+apply (erule exE)
+apply (drule_tac f="%x. Nat2nat(x)" in arg_cong)
+apply (simp (no_asm_use) only: Nat2nat_mul iso2)
+apply (auto)
+done
+
+
+theorem Nat2nat_dvd : "(Nat2nat(x) dvd Nat2nat(y)) = (x dvd' y)"
+apply (auto)
+apply (subst (asm) nat2Nat_dvd [THEN sym])
+apply (auto)
+done
+
+section "Simple Functions"
+
+theorem nat2Nat_max [simp]: "nat2Nat(max x y) = max'(nat2Nat(x),nat2Nat(y))"
+apply (simp add: max_def_Nat max_def)
+done
+
+theorem Nat2nat_max : "Nat2nat(max'(x,y)) = (max (Nat2nat(x)) (Nat2nat(y)))"
+apply (simp add: max_def_Nat max_def)
+done
+
+theorem nat2Nat_min : "nat2Nat(min x y) = min' (nat2Nat(x), nat2Nat(y))"
+apply (simp add: min_def_Nat min_def)
+done
+
+theorem Nat2nat_min : "Nat2nat(min'(x,y)) = (min (Nat2nat(x)) (Nat2nat(y)))"
+apply (simp add: min_def_Nat min_def)
+done
+
+
+(* ============================================================================= *)
+(* ============================== cut off minus ================================ *)
+(* ============================================================================= *)
+
+
+lemma anything_part_minus_zero [simp] : "x -? 0' = makePartial x"
+apply (simp add: sub_def_Nat)
+done
+
+lemma add_partiality  : "x=y <-> makePartial x = makePartial y"
+apply (simp add: makePartial_def)
+done
+
+
+lemma anything_minus_zero [simp] : "x -! 0' = x"
+(* here the problem is that the defined rewrite rule is only applicable for makePartial x-!y *)
+apply (subst add_partiality)
+apply (subst subTotal_def2_Nat)
+apply (simp)
+apply (subst anything_part_minus_zero)
+apply (simp)
+done
+
+lemma not_greater_zero : "~ x>'0' <-> x <=' 0'"
+apply (simp)
+apply (auto)
+done
+
+
+
+lemma zero_minus_anything [simp] : "0' -! x = 0'"
+apply (case_tac "x>'0'")
+apply (simp only: subTotal_def1_Nat)
+apply (subst (asm) not_greater_zero)
+apply (subst add_partiality)
+apply (subst subTotal_def2_Nat)
+apply (auto)
+done
+
+lemma not_iff : "(A<->B) <-> (~A <-> ~B)"
+apply (auto)
+done
+
+
+lemma not_greater_suc : "~ (x>'y) <-> x <' X_suc(y)"
+apply (insert Nat2nat_gt)
+apply (subst (asm) not_iff)
+apply (subst (asm) not_less_eq)
+apply (subst (asm) Nat2nat_suc [rule_format, THEN sym])
+apply (subst (asm) Nat2nat_lt )
+apply (auto)
+done
+
+lemma not_greater_isa : "~((x::nat) > (y::nat)) <-> x<=y"
+apply (arith)
+done
+
+lemma minus_Suc : "(Suc(x) - Suc(y))=(x-y)"
+apply (auto)
+done
+
+lemma not_greater : " ~ (x>'y) <-> x<='y"
+sorry
+
+lemma minus_neutral : "(x <=' y) ==> y = (y -! x) +' x"
+apply (drule subTotal_def2_Nat)
+apply (drule sym)
+apply (subst (asm) sub_def_Nat)
+apply (auto)
+done
+
+(*forward reasoning anstatt makePartial einfügen ist hilfreich*)
+
+lemma minus_suc : "(X_suc(x) -! X_suc(y))=(x-!y)"
+apply (case_tac "y>'x")
+apply (simp)
+apply (subst (asm) not_greater)
+apply (subst add_partiality)
+apply (subst subTotal_def2_Nat)
+apply (simp)
+apply (subst sub_def_Nat)
+apply (subst ga_comm___XPlus__)
+apply (subst add_suc_Nat)
+apply (subst ga_injective_suc)
+apply (subst ga_comm___XPlus__)
+apply (rule minus_neutral)
+apply (simp)
+done
+
+theorem nat2Nat_minus: "nat2Nat (x - y) = (nat2Nat(x) -! nat2Nat (y))"
+apply (rule diff_induct)
+apply (simp)
+apply (simp only: nat2Nat_0 nat2Nat_Suc diff_0_eq_0 zero_minus_anything)
+apply (subst minus_Suc)
+apply (simp)
+apply (subst minus_suc)
+apply (auto)
+done
+
+theorem Nat2nat_minus: "Nat2nat (x -! y) = (Nat2nat (x) - Nat2nat(y))"
+apply (rule nat2Nat_injectivity)
+apply (subst nat2Nat_minus)
+apply (auto)
+done
+
+
+section "Partial Functions"
+
+theorem iso2_negated: "~(nat2Nat(x)=nat2Nat(y)) ==> ~(x=y)"
+apply (auto)
+done
+
+theorem iso1_negated1: "x~=y ==> ~(Nat2nat(x)=Nat2nat(y))"
+apply (auto)
+apply (drule Nat2nat_injectivity)
+apply (auto)
+done
+
+
+
+
+
+section "Non-canonical Mappings"
+
+theorem nat2Nat_at : "nat2Nat(x @@@ y) = nat2Nat(x) @@ nat2Nat(y)"
+apply (auto simp add: decimal_def decimal_def_nat)
+apply (rule Nat2nat_injectivity)
+apply (simp only: Nat2nat_mul Nat2nat_add Nat2nat_9_def_Nat[rule_format, THEN sym])
+by (auto)
+
+theorem Nat2nat_at  : "Nat2nat( x @@ y) = Nat2nat(x) @@@ Nat2nat(y)"
+apply (simp only: decimal_def decimal_def_nat)
+apply (simp only: Nat2nat_mul Nat2nat_suc Nat2nat_add Nat2nat_9_def_Nat[rule_format, THEN sym])
+done
+
+
+theorem Nat2nat_pre : "!!x. x > 0 ==> nat2Nat(makeTotal(pre_nat(x))) = makeTotal(pre(nat2Nat(x)))"
+(* moeglichst schnell definition von pre einsetzen *)
+apply (case_tac x)
+apply (simp)
+apply (simp add: ga_selector_pre nat2Nat_Suc)
+done
+
+theorem nat2Nat_pre : "x >' 0' ==> Nat2nat(makeTotal(pre(x))) = makeTotal(pre_nat(Nat2nat(x)))"
+apply (subst (asm) Nat2nat_gt[THEN sym])
+apply (simp only: Nat2nat_0)
+apply (rule nat2Nat_injectivity)
+apply (subst Nat2nat_pre)
+apply (simp)
+apply (simp add: iso2)
+done
+
+lemma makepartial_intro_weak: "(s=makePartial t) ==> (makeTotal(s)=t)"
+apply (simp add: makePartial_def makeTotal_def)
+done
+
+theorem nat2Nat_div [simp]: "y ~= 0 ==> nat2Nat(x div y) = makeTotal(nat2Nat(x) div' nat2Nat(y))"
+apply (rule sym)
+apply (rule makepartial_intro_weak)
+apply (subst div_Nat)
+apply (rule_tac x="nat2Nat (x mod y)" in exI)
+apply (rule conjI)
+apply (rule Nat2nat_injectivity)
+apply (simp only: iso2 Nat2nat_add Nat2nat_mul)
+apply (arith)
+apply (subst nat2Nat_lt)
+apply (rule mod_less_divisor)
+apply (arith)
+done
+
+theorem Nat2nat_div : " y ~= 0' ==> Nat2nat(makeTotal (x div' y)) = Nat2nat(x) div Nat2nat(y)"
+apply (frule iso1_negated1)
+apply (subst (asm) Nat2nat_0)
+apply (rule nat2Nat_injectivity)
+apply (simp)
+done
+
+theorem nat2Nat_mod [simp] : "~(y = 0) ==> nat2Nat(x mod y) =makeTotal (nat2Nat(x) mod' nat2Nat(y))"
+apply (rule sym)
+apply (rule makepartial_intro_weak)
+(*apply (subst nat2Nat_mod_mp[rule_format,THEN sym])*)
+apply (simp)
+apply (subst mod_Nat)
+apply (rule_tac x="nat2Nat (x div y)" in exI)
+apply (rule conjI)
+apply (subst nat2Nat_mul[rule_format,THEN sym])
+apply (subst nat2Nat_add[rule_format,THEN sym])
+apply (rule_tac f="nat2Nat" in arg_cong)
+apply (simp)
+apply (subst Nat2nat_lt[THEN sym])
+apply (simp only: iso2)
+apply (rule mod_less_divisor)
+apply (auto)
+done
+
+theorem Nat2nat_mod : "~(y = 0') ==>  Nat2nat (makeTotal (x mod' y)) = (Nat2nat(x) mod Nat2nat(y))"
+apply (frule iso1_negated1)
+apply (subst (asm) Nat2nat_0)
+apply (rule nat2Nat_injectivity)
+apply (simp)
+done
+
+theorem nat2Nat_pdiv : "[|~ y = 0 ; x mod y = 0|] ==> nat2Nat(makeTotal(x /?? y)) =makeTotal(nat2Nat(x) /? nat2Nat(y))"
+apply (rule sym)
+apply (rule makepartial_intro_weak)
+apply (subst divide_Nat_Nat)
+apply (subst Nat2nat_gt[THEN sym])
+apply (simp)
+apply (rule Nat2nat_injectivity)
+apply (simp only: Nat2nat_mul iso2)
+apply (subst part_div_def)
+apply (simp)
+apply (auto)
+done
+
+theorem Nat2nat_pdiv : "[|~ y = 0' ; x mod' y = makePartial 0'|] ==> Nat2nat(makeTotal(x /? y)) =makeTotal(Nat2nat(x) /?? Nat2nat(y))"
+apply (drule iso1_negated1)
+apply (subst (asm) Nat2nat_0)
+apply (drule_tac f="%x. makeTotal(x)" in arg_cong)
+apply (drule_tac f="%x. Nat2nat(x)" in arg_cong)
+apply (simp only: makePartialproj)
+apply (subst (asm) Nat2nat_mod)
+apply (rule Nat2nat_injectivity_negated)
+apply (simp)
+apply (simp  only: makePartialproj Nat2nat_0 Nat2nat_mod)
+apply (rule nat2Nat_injectivity)
+apply (drule nat2Nat_pdiv)
+apply (simp)
+apply (simp)
+done
+
+theorem nat2Nat_pminus : "(x >= y) ==> nat2Nat(makeTotal (x -?? y)) = makeTotal(nat2Nat(x) -? nat2Nat(y))"
+apply (rule sym)
+apply (rule makepartial_intro_weak)
+apply (subst sub_def_Nat)
+apply (rule Nat2nat_injectivity)
+apply (simp only: Nat2nat_add iso2)
+apply (subst part_minus_def)
+apply (simp add: makePartialproj)
+done
+
+theorem Nat2nat_pminus : "(x >=' y) ==> Nat2nat(makeTotal(x -? y)) = makeTotal(Nat2nat(x) -?? Nat2nat(y))"
+apply (subst (asm) Nat2nat_gt_equal[THEN sym])
+apply (rule nat2Nat_injectivity)
+apply (subst nat2Nat_pminus)
+apply (simp)
+apply (simp)
+done
 
 end
